Update AES semantics to be compatible with compiler proofs (#800)

investigations/bedrock2/Aes/AesProperties.v
@@ -19,6 +19,7 @@ Require Import coqutil.Map.Properties.
 Require Import coqutil.Tactics.Tactics.
 Require Import coqutil.Tactics.syntactic_unify.
 Require Import coqutil.Tactics.letexists.
+Require Import coqutil.Z.Lia.
 Require Import Cava.Util.List.
 Require Import Cava.Util.Tactics.
 Require Import Bedrock2Experiments.StateMachineSemantics.
@@ -66,190 +67,21 @@ Section Proofs.
     change Semantics.word_ok with parameters.word_ok in *;
     change Semantics.mem_ok with parameters.mem_ok in *.
 
-  Hint Extern 4 (step _ ?s _ _ _) =>
-  eapply (ReadStep (p:=state_machine_parameters) s) : step.
-  Hint Extern 4 (step _ ?s _ _ _) =>
-  eapply (WriteStep (p:=state_machine_parameters) s) : step.
-
-  Lemma word_add_0_r (w : parameters.word) : word.add w (word.of_Z 0) = w.
-  Proof. ring. Qed.
-
-  Lemma reg_addr_unique r1 r2 : reg_addr r1 = reg_addr r2 -> r1 = r2.
-  Proof.
-    pose proof addrs_unique as Huniq.
-    cbv [aes_reg_addrs list_reg_addrs] in *.
-    rewrite nregs_key_eq, nregs_iv_eq, nregs_data_eq in Huniq.
-    repeat lazymatch type of Huniq with
-           | context [Z.to_nat ?n] =>
-             let x := constr:(Z.to_nat n) in
-             let y := (eval vm_compute in x) in
-             change x with y in Huniq
-           | _ => progress cbn [seq map app] in Huniq
-           end.
-    simplify_unique_words_in Huniq.
-    rewrite !word_add_0_r in *.
-    cbv [reg_addr]; cbn; intro Heqaddr.
-    destruct r1.
-    (* clear all hypothesis that don't have to do with r1 (makes proof
-       faster) *)
-    all:lazymatch type of Heqaddr with
-        | ?r = _ =>
-          repeat match goal with
-                 | H : ?x <> ?y |- _ =>
-                   lazymatch x with
-                   | context [r] => fail
-                   | _ =>
-                     lazymatch y with
-                     | context [r] => fail
-                     | _ => clear H
-                     end
-                   end
-                 end
-        end.
-    all:destruct r2; try first [ exact eq_refl | congruence ].
-  Qed.
-
-  (* alternate form of reg_addr_unique *)
-  Lemma reg_addr_neq r1 r2 : r1 <> r2 -> reg_addr r1 <> reg_addr r2.
-  Proof.
-    intros. intro Heq. apply reg_addr_unique in Heq. congruence.
-  Qed.
-
-  (* TODO: move to Util/List *)
-  Lemma existsb_nexists {A} (f : A -> bool) l : existsb f l = false <-> (forall x, In x l -> f x = false).
-  Proof.
-    split.
-    { induction l; intros; cbn [In existsb] in *; [ tauto | ].
-      repeat lazymatch goal with
-             | H : (_ || _)%bool = false |- _ => apply Bool.orb_false_iff in H; destruct H
-             | H : _ \/ _ |- _ => destruct H
-             | _ => subst; eauto; congruence
-             end. }
-    { induction l; intros; cbn [In existsb] in *; [ tauto | ].
-      rewrite IHl by auto. rewrite Bool.orb_false_r. eauto. }
-  Qed.
-
-  Lemma addr_in_category_reg_addr r c :
-    addr_in_category (reg_addr r) c = reg_category_eqb c (reg_category r).
-  Proof.
-    cbv [addr_in_category].
-    case_eq (reg_category_eqb c (reg_category r)); intros.
-    { apply existsb_exists; exists r.
-      split; [ apply all_regs_complete | ].
-      apply Bool.andb_true_iff; split; [ apply word.eqb_eq; reflexivity | ].
-      congruence. }
-    { apply existsb_nexists; intro r2. intros.
-      apply Bool.andb_false_iff.
-      destr (word.eqb (reg_addr r) (reg_addr r2)).
-      { lazymatch goal with
-          H : reg_addr _ = reg_addr _ |- _ => apply reg_addr_unique in H end.
-        subst. tauto. }
-      { left. apply word.eqb_ne; auto. } }
-  Qed.
-
-  Lemma nregs_populated_put rs r v cat :
-    reg_lookup rs r = None ->
-    nregs_populated (map.put rs (reg_addr r) v) cat =
-    if reg_category_eqb cat (reg_category r)
-    then S (nregs_populated rs cat)
-    else nregs_populated rs cat.
-  Proof.
-    cbv [nregs_populated reg_lookup]. intros.
-    rewrite map.fold_put; auto.
-    { rewrite addr_in_category_reg_addr. reflexivity. }
-    { intros. repeat destruct_one_match; reflexivity. }
-  Qed.
-
-  Lemma nregs_populated_remove rs r cat v :
-    reg_lookup rs r = Some v ->
-    nregs_populated (map.remove rs (reg_addr r)) cat =
-    if reg_category_eqb cat (reg_category r)
-    then (nregs_populated rs cat - 1)%nat
-    else nregs_populated rs cat.
-  Proof.
-    cbv [nregs_populated reg_lookup]. intros.
-    erewrite map.fold_remove with (m:=rs); eauto; [ | ].
-    { rewrite addr_in_category_reg_addr.
-      destruct_one_match; try reflexivity. lia. }
-    { intros. repeat destruct_one_match; reflexivity. }
-  Qed.
-
-  Lemma regs_empty_impl rs c r :
-    nregs_populated rs c = 0%nat ->
-    reg_category_eqb c (reg_category r) = true ->
-    reg_lookup rs r = None.
-  Proof.
-    intros. revert dependent rs.
-    cbv [nregs_populated].
-    apply (map.fold_spec (fun rs count => count = 0%nat -> reg_lookup rs r = None));
-      intros; [ apply map.get_empty | ].
-    cbv [reg_lookup] in *.
-    destruct_one_match_hyp; try congruence; [ ].
-    rewrite map.get_put_dec.
-    destruct_one_match; subst; [ | tauto ].
-    rewrite addr_in_category_reg_addr in *.
-    congruence.
-  Qed.
-
-  Lemma regs_lookup_put rs r1 r2 v :
-    r1 <> r2 -> reg_lookup rs r1 = None ->
-    reg_lookup (map.put rs (reg_addr r2) v) r1 = None.
-  Proof.
-    cbv [reg_lookup]. intros.
-    rewrite map.get_put_diff by (apply reg_addr_neq; congruence).
-    assumption.
-  Qed.
-
-  Lemma unset_inp_regs_put rs r v :
-    unset_inp_regs (map.put rs (reg_addr r) v) =
-    if (reg_category_eqb DataInReg (reg_category r)
-        || reg_category_eqb IVReg (reg_category r)
-        || reg_category_eqb KeyReg (reg_category r))%bool
-    then unset_inp_regs rs
-    else map.put (unset_inp_regs rs) (reg_addr r) v.
-  Proof.
-    cbv [unset_inp_regs]. apply map.map_ext; intros.
-    destruct_one_match.
-    { rewrite !map.get_remove_dec.
-      repeat (destruct_one_match; try reflexivity); [ ].
-      apply map.get_put_diff.
-      destruct r; cbn [reg_category reg_category_eqb orb] in *; congruence. }
-    { repeat lazymatch goal with H : (_ || _)%bool = false |- _ =>
-                                 apply Bool.orb_false_iff in H; destruct H end.
-      repeat lazymatch goal with
-               | |- context [map.get (map.put _ _ _) _] => rewrite map.get_put_dec
-               | |- context [map.get (map.remove _ _) _] => rewrite map.get_remove_dec
-               | H : reg_addr _ = reg_addr _ |- _ =>
-                 apply reg_addr_unique in H; subst;
-                   cbn [reg_category reg_category_eqb] in *; try congruence
-               | _ => destruct_one_match; subst; try reflexivity
-               end. }
-  Qed.
-
-  (* tactic to feed to [interaction] which will solve the side conditions of
-     interact_mmio *)
-  Local Ltac solve_dexprs :=
+  (* tactic to solve the side conditions of interact_read and interact_write *)
+  Local Ltac solve_dexprs ::=
     repeat straightline_with_map_lookup;
     simplify_implicits; repeat straightline_with_map_lookup.
 
-  (* run [interaction] and then assert the register's identity *)
-  Local Ltac interaction_with_reg R :=
-    (* this simplification step ensures that the parameters.reg_addr hypothesis
-       we see is a new one *)
-    cbn [parameters.reg_addr parameters.write_step parameters.read_step
-                             state_machine_parameters] in *;
-    interaction solve_dexprs;
-    simplify_implicits;
-    (* assert that the register address matches R *)
-    lazymatch goal with
-    | H : parameters.reg_addr ?r = ?addr |- _ =>
-      replace addr with (reg_addr R) in H
-        by (cbn [reg_addr]; subst_lets; ring);
-      apply reg_addr_unique in H; try subst r
-    end;
-    (* simplify again *)
-    cbn [parameters.reg_addr parameters.write_step parameters.read_step
-                             state_machine_parameters] in *.
+  (* tactic to simplify side conditions in terms of [dexpr] *)
+  Local Ltac dexpr_hammer :=
+    subst_lets; simplify_implicits;
+    repeat first [ progress push_unsigned
+                 | rewrite word.unsigned_of_Z in *
+                 | rewrite word.wrap_small in * by lia
+                 | destruct_one_match
+                 | lia
+                 | progress ring_simplify
+                 | reflexivity ].
 
   Lemma execution_unique (t : trace) s1 s2 :
     execution t s1 ->
@@ -266,22 +98,26 @@ Section Proofs.
     | H1 : execution t ?s1, H2 : execution t ?s2 |- _ =>
       specialize (IHt _ _ H1 H2); subst
     end.
-    repeat invert_step; subst;
-      repeat lazymatch goal with
-             | H : _ :: _ = _ :: _ |- _ => inversion H; clear H; subst
-             end;
-      cbn [parameters.read_step parameters.write_step
-                                parameters.reg_addr
-                                state_machine_parameters] in *;
-      cbv [read_step write_step] in *.
-    all: repeat lazymatch goal with
-                | H : False |- _ => contradiction H
-                | H : _ /\ _ |- _ => destruct H
-                | H : _ = reg_addr _ |- _ => apply reg_addr_unique in H; subst
-                | |- ?x = ?x => reflexivity
-                | _ => first [ progress subst
-                            | destruct_one_match_hyp ]
-                end.
+    cbv [step] in *. cbn [ parameters.read_step
+                             parameters.write_step
+                             state_machine_parameters] in *.
+    repeat destruct_one_match_hyp; try congruence; [ | ].
+    all:logical_simplify; subst.
+    all: lazymatch goal with
+         | H : parameters.reg_addr ?x = parameters.reg_addr ?y |- _ =>
+           eapply (parameters.reg_addr_unique
+                     (ok:=state_machine_parameters_ok) x y) in H
+         end.
+    all:cbv [write_step read_step] in *; subst.
+    all:repeat destruct_one_match_hyp; try congruence.
+    all:logical_simplify; subst.
+    all:lazymatch goal with
+        | H : False |- _ => contradiction H
+        | H1 : ?x = Some ?a, H2 : ?x = Some ?b |- _ =>
+          rewrite H1 in H2; inversion H2; clear H2; subst
+        | _ => idtac
+        end.
+    all:reflexivity.
   Qed.
 
   Local Ltac infer_states_equal :=
@@ -298,49 +134,394 @@ Section Proofs.
            | H : DONE _ = DONE _ |- _ => inversion H; clear H; subst
            end.
 
-  Local Ltac invert_read_step :=
-    lazymatch goal with
-    | H : read_step _ _ _ _ |- _ =>
-      cbv [read_step] in H; cbn [reg_category] in H
-    end;
-    logical_simplify; simplify_implicits;
-    repeat lazymatch goal with
-           | H : False |- _ => contradiction H
-           | Heq : nregs_populated _ ?c = _,
-                   H : context [nregs_populated (map.remove ?m _) ?c] |- _ =>
-             erewrite !nregs_populated_remove in H by eauto;
-               simplify_implicits; rewrite Heq in H;
-                 cbn [reg_category reg_category_eqb Nat.sub] in H
-           | H : S _ = O |- _ => lia
-           | H : O <> O |- _ => lia
-           | _ => first [ destruct_one_match_hyp
-                       | progress logical_simplify ]
-           end.
-
-  Local Ltac invert_write_step :=
-    lazymatch goal with
-    | H : write_step _ _ _ _ |- _ =>
-      cbv [write_step] in H; cbn [reg_category] in H
-    end;
-    repeat lazymatch goal with
-           | Hemp : nregs_populated _ ?c = 0%nat,
-                    H : context [nregs_populated (map.put _ _ _) ?c] |- _ =>
-             rewrite !nregs_populated_put in H
-               by (repeat (apply regs_lookup_put; [ congruence | ]);
-                   eauto using regs_empty_impl);
-             rewrite Hemp in H;
-             cbn [reg_category reg_category_eqb Nat.eqb] in H; subst
-           | H : False |- _ => contradiction H
-           | _ => first [ destruct_one_match_hyp
-                       | progress logical_simplify ]
-           end.
-
   Local Ltac infer :=
     repeat first [ progress infer_states_equal
-                 | progress infer_state_data_equal
-                 | progress invert_read_step; [ ]
-                 | progress invert_write_step; [ ]
-                 | progress invert_step ].
+                 | progress infer_state_data_equal ].
+
+  (* TODO: lots of annoying bit arithmetic here, maybe try to clean it up *)
+  Lemma status_read_always_ok s :
+    exists val s', read_step s STATUS val s'.
+  Proof.
+    assert (forall x y : parameters.word,
+               word.slu (word.of_Z 1) x <> word.slu (word.of_Z 1) y -> x <> y)
+           as Hshift_neq by (intros; subst; congruence).
+    pose proof status_flags_unique_and_nonzero as Hflags.
+    simplify_unique_words_in Hflags.
+    repeat match goal with
+           | H : _ |- _ => apply Hshift_neq in H
+           end.
+    pose proof status_flags_inbounds as Hbounds.
+    repeat lazymatch goal with
+           | H : Forall _ (_ :: _) |- _ =>
+             pose proof (Forall_inv H);
+               apply Forall_inv_tail in H
+           | H : Forall _ [] |- _ => clear H
+           end.
+    cbv beta in *.
+    destruct s; cbn [read_step reg_category status_matches_state].
+    { exists (word.of_Z 0). eexists; ssplit; [ | reflexivity ].
+      cbv [is_flag_set]. boolsimpl.
+      rewrite !word.eqb_eq; [ reflexivity | apply word.unsigned_inj .. ].
+      all:push_unsigned; rewrite Z.land_0_l; reflexivity. }
+    { exists (word.or (word.slu (word.of_Z 1) AES_STATUS_IDLE)
+                 (word.slu (word.of_Z 1) AES_STATUS_INPUT_READY)).
+      eexists; ssplit; [ | reflexivity ].
+      cbv [is_flag_set]. boolsimpl.
+      repeat lazymatch goal with
+             | |- (_ && _)%bool = true => apply Bool.andb_true_iff; split
+             | |- negb _ = true => apply Bool.negb_true_iff
+             end.
+      all:rewrite word.unsigned_eqb.
+      all:first [ apply Z.eqb_eq | apply Z.eqb_neq ].
+      all:try lazymatch goal with
+              | |- word.unsigned (word.and ?x ?y) <> _ =>
+                let H := fresh in
+                assert (word.unsigned (word.and x y) = word.unsigned y)
+                  as H;
+                  [ | rewrite H; intro Heq; apply word.unsigned_inj in Heq;
+                      simplify_implicits; cbn in *; congruence ]
+              end.
+      all:push_unsigned; cbv [word.wrap]; rewrite <-!Z.land_ones by lia;
+        bitblast.Z.bitblast.
+      all:rewrite !Z_testbit_1_l;
+        repeat lazymatch goal with
+               | |- context [?x =? ?y] =>
+                 destr (x =? y)
+               end.
+      all:boolsimpl; try reflexivity.
+      all:subst.
+      all:lazymatch goal with
+          | H1 : ?i - word.unsigned ?x = 0,
+                 H2 : ?i - word.unsigned ?y = 0 |- _ =>
+            assert (x = y) by (apply word.unsigned_inj; lia)
+          end.
+      all:simplify_implicits; cbn in *; congruence. }
+    { exists (word.slu (word.of_Z 1) AES_STATUS_OUTPUT_VALID).
+      destruct data. rewrite is_flag_set_shift by (cbv [boolean]; tauto || lia).
+      rewrite word.eqb_ne by
+          (intro Heq; apply word.of_Z_inj_small in Heq; lia).
+      cbn [negb]. eauto. }
+    { exists (word.slu (word.of_Z 1) AES_STATUS_OUTPUT_VALID).
+      eexists; split; [ | reflexivity ].
+      rewrite is_flag_set_shift by (cbv [boolean]; tauto || lia).
+      rewrite word.eqb_ne by
+          (intro Heq; apply word.of_Z_inj_small in Heq; lia).
+      rewrite !is_flag_set_shift_neq by
+          (cbv [boolean];
+           first [ tauto | lia
+                   | intro; cbn in *; simplify_implicits; congruence ]).
+      reflexivity. }
+  Qed.
+
+  (* solve common side conditions from interactions *)
+  Local Ltac post_interaction :=
+    lazymatch goal with
+    | |- dexprs _ _ _ _ => solve_dexprs; reflexivity
+    | |- reg_addr _ = _ => reflexivity
+    | |- execution _ _ => eassumption
+    | |- ?G => tryif is_lia G then lia else eauto
+    end.
+
+  Lemma interact_read_status s call bind addre t m l
+        (post : trace -> mem -> locals -> Prop) addr :
+    dexprs m l [addre] [addr] ->
+    reg_addr STATUS = addr ->
+    execution t s ->
+    (forall s' val,
+        read_step s STATUS val s' ->
+        (* implied by other preconditions but convenient to have separately *)
+        execution ((map.empty, READ, [addr], (map.empty, [val])) :: t) s' ->
+        post ((map.empty, READ, [addr], (map.empty, [val])) :: t)
+             m (map.put l bind val)) ->
+    cmd call (cmd.interact [bind] READ [addre]) t m l post.
+  Proof.
+    intros; eapply interact_read; intros; infer;
+      cbv [parameters.read_step state_machine_parameters] in *;
+      eauto.
+    pose proof status_read_always_ok s. logical_simplify.
+    do 3 eexists; eauto.
+  Qed.
+
+  Lemma interact_write_control s call addre vale t m l
+        (post : trace -> mem -> locals -> Prop) addr val :
+    dexprs m l [addre; vale] [addr; val] ->
+    reg_addr CTRL = addr ->
+    execution t s ->
+    match s with
+    | IDLE _ => True
+    | UNINITIALIZED => True
+    | _ => False
+    end ->
+    (forall s',
+        write_step s CTRL val s' ->
+        (* implied by other preconditions but convenient to have separately *)
+        execution ((map.empty, WRITE, [addr;val], (map.empty, [])) :: t) s' ->
+        post ((map.empty, WRITE, [addr;val], (map.empty, [])) :: t)
+             m l) ->
+    cmd call (cmd.interact [] WRITE [addre;vale]) t m l post.
+  Proof.
+    intros; eapply interact_write; intros; infer;
+      cbv [parameters.write_step state_machine_parameters] in *;
+      eauto.
+    cbv [write_step]. cbn [reg_category].
+    exists s; destruct s; try contradiction;
+      repeat destruct_one_match;
+      eexists; ssplit; (assumption || reflexivity).
+  Qed.
+
+  Definition key_from_index (i : nat) : Register :=
+    nth i [KEY0;KEY1;KEY2;KEY3;KEY4;KEY5;KEY6;KEY7] CTRL.
+
+  Lemma key_from_index_category i :
+    (i < 8)%nat -> reg_category (key_from_index i) = KeyReg.
+  Proof.
+    intros. cbv [key_from_index].
+    apply Forall_nth; [ |  length_hammer ].
+    repeat constructor.
+  Qed.
+
+  Lemma interact_write_key i call addre vale t m l
+        (post : trace -> mem -> locals -> Prop) rs addr val :
+    dexprs m l [addre; vale] [addr; val] ->
+    addr = word.add AES_KEY0 (word.mul (word.of_Z (Z.of_nat i)) (word.of_Z 4)) ->
+    (i < 8)%nat ->
+    execution t (IDLE rs) ->
+    (forall s',
+        write_step (IDLE rs) (key_from_index i) val s' ->
+        (* implied by other preconditions but convenient to have separately *)
+        execution ((map.empty, WRITE, [addr;val], (map.empty, [])) :: t) s' ->
+        post ((map.empty, WRITE, [addr;val], (map.empty, [])) :: t)
+             m l) ->
+    cmd call (cmd.interact [] WRITE [addre;vale]) t m l post.
+  Proof.
+    intros; eapply interact_write; intros; infer;
+      cbv [parameters.write_step state_machine_parameters] in *;
+      eauto.
+    { repeat (destruct i; try lia); subst; cbn; ring. }
+    { cbv [write_step]. rewrite key_from_index_category by lia.
+      exists (IDLE rs). eexists; ssplit; eauto. }
+  Qed.
+
+  Definition iv_from_index (i : nat) : Register :=
+    nth i [IV0;IV1;IV2;IV3] CTRL.
+
+  Lemma iv_from_index_category i :
+    (i < 4)%nat -> reg_category (iv_from_index i) = IVReg.
+  Proof.
+    intros. cbv [iv_from_index].
+    apply Forall_nth; [ | length_hammer ].
+    repeat constructor.
+  Qed.
+
+  Lemma interact_write_iv i call addre vale t m l
+        (post : trace -> mem -> locals -> Prop) rs addr val :
+    dexprs m l [addre; vale] [addr; val] ->
+    addr = word.add AES_IV0 (word.mul (word.of_Z (Z.of_nat i)) (word.of_Z 4)) ->
+    (i < 4)%nat ->
+    execution t (IDLE rs) ->
+    (forall s',
+        write_step (IDLE rs) (iv_from_index i) val s' ->
+        (* implied by other preconditions but convenient to have separately *)
+        execution ((map.empty, WRITE, [addr;val], (map.empty, [])) :: t) s' ->
+        post ((map.empty, WRITE, [addr;val], (map.empty, [])) :: t)
+             m l) ->
+    cmd call (cmd.interact [] WRITE [addre;vale]) t m l post.
+  Proof.
+    intros; eapply interact_write; intros; infer;
+      cbv [parameters.write_step state_machine_parameters] in *;
+      eauto.
+    { repeat (destruct i; try lia); subst; cbn; ring. }
+    { cbv [write_step]. rewrite iv_from_index_category by lia.
+      exists (IDLE rs). eexists; ssplit; eauto. }
+  Qed.
+
+  Definition data_in_from_index (i : nat) : Register :=
+    nth i [DATA_IN0;DATA_IN1;DATA_IN2;DATA_IN3] CTRL.
+
+  Lemma data_in_from_index_category i :
+    (i < 4)%nat -> reg_category (data_in_from_index i) = DataInReg.
+  Proof.
+    intros. cbv [data_in_from_index].
+    apply Forall_nth; [ | length_hammer ].
+    repeat constructor.
+  Qed.
+
+  Lemma interact_write_data_in i call addre vale t m l
+        (post : trace -> mem -> locals -> Prop) rs addr val :
+    dexprs m l [addre; vale] [addr; val] ->
+    addr = word.add AES_DATA_IN0 (word.mul (word.of_Z (Z.of_nat i)) (word.of_Z 4)) ->
+    (i < 4)%nat ->
+    execution t (IDLE rs) ->
+    (forall s',
+        write_step (IDLE rs) (data_in_from_index i) val s' ->
+        (* implied by other preconditions but convenient to have separately *)
+        execution ((map.empty, WRITE, [addr;val], (map.empty, [])) :: t) s' ->
+        post ((map.empty, WRITE, [addr;val], (map.empty, [])) :: t)
+             m l) ->
+    cmd call (cmd.interact [] WRITE [addre;vale]) t m l post.
+  Proof.
+    intros; eapply interact_write; intros; infer;
+      cbv [parameters.write_step state_machine_parameters] in *;
+      eauto.
+    { repeat (destruct i; try lia); subst; cbn; ring. }
+    { cbv [write_step]. rewrite data_in_from_index_category by lia.
+      exists (IDLE rs). destruct_one_match; eexists; ssplit; eauto. }
+  Qed.
+
+
+  Definition data_out_from_index (i : nat) : Register :=
+    nth i [DATA_OUT0;DATA_OUT1;DATA_OUT2;DATA_OUT3] CTRL.
+
+  Lemma data_out_from_index_category i :
+    (i < 4)%nat -> reg_category (data_out_from_index i) = DataOutReg.
+  Proof.
+    intros. cbv [data_out_from_index].
+    apply Forall_nth; [ | length_hammer ].
+    repeat constructor.
+  Qed.
+
+  Lemma interact_read_data_out i call addre bind t m l
+        (post : trace -> mem -> locals -> Prop) data addr val :
+    dexprs m l [addre] [addr] ->
+    addr = word.add AES_DATA_OUT0 (word.mul (word.of_Z (Z.of_nat i)) (word.of_Z 4)) ->
+    (i < 4)%nat ->
+    match data_out_from_index i with
+    | DATA_OUT0 => done_data_out0 data
+    | DATA_OUT1 => done_data_out1 data
+    | DATA_OUT2 => done_data_out2 data
+    | DATA_OUT3 => done_data_out3 data
+    | _ => None
+    end = Some val ->
+    execution t (DONE data) ->
+    (forall s' val,
+        read_step (DONE data) (data_out_from_index i) val s' ->
+        (* implied by other preconditions but convenient to have separately *)
+        execution ((map.empty, READ, [addr], (map.empty, [val])) :: t) s' ->
+        post ((map.empty, READ, [addr], (map.empty, [val])) :: t)
+             m (map.put l bind val)) ->
+    cmd call (cmd.interact [bind] READ [addre]) t m l post.
+  Proof.
+    intros; eapply interact_read with (r:=data_out_from_index i);
+      intros; infer;
+        cbv [parameters.read_step state_machine_parameters] in *;
+        eauto.
+    { repeat (destruct i; try lia); subst; cbn; ring. }
+    { cbv [read_step]. rewrite data_out_from_index_category by lia.
+      exists (DONE data). repeat (destruct i; try lia); subst.
+      all:cbn [data_out_from_index nth read_output_reg] in *.
+      all:match goal with H : _ = Some _ |- _ => rewrite H end.
+      all:do 2 eexists; ssplit; eauto. }
+  Qed.
+
+  Lemma get_aes_input_none data :
+    (idle_data_in0 data = None
+     \/ idle_data_in1 data = None
+     \/ idle_data_in2 data = None
+     \/ idle_data_in3 data = None) ->
+    get_aes_input data = None.
+  Proof.
+    cbv [get_aes_input]. destruct data; cbn; intros.
+    repeat lazymatch goal with
+           | H : _ \/ _ |- _ => destruct H
+           | H : ?x = None |- _ => rewrite H
+           end.
+    all:repeat destruct_one_match; reflexivity.
+  Qed.
+
+  (* apply interact_read_status and do some post-processing *)
+  Local Ltac read_status :=
+    eapply interact_read_status; [ try post_interaction .. | ].
+
+  (* apply interact_write_status and do some post-processing *)
+  Local Ltac write_control :=
+    eapply interact_write_control; [ try post_interaction .. | ].
+
+  (* apply interact_write_key and do some post-processing *)
+  Local Ltac write_key :=
+    eapply interact_write_key;
+    [ try post_interaction ..
+    | intros;
+      try lazymatch goal with
+          | H : write_step _ _ _ _ |- _ =>
+            cbv [write_step] in H;
+            rewrite key_from_index_category in H by lia; subst
+          end ].
+
+  (* apply interact_write_iv for the nth IV register, and do some
+     post-processing *)
+  Local Ltac write_iv_n n :=
+    eapply interact_write_iv with (i:=n);
+    [ try post_interaction ..
+    | intros;
+      try lazymatch goal with
+          | H : write_step _ _ _ _ |- _ =>
+            cbv [write_step] in H;
+            rewrite iv_from_index_category in H by lia; subst
+          end ].
+
+  (* apply interact_write_data_in for the nth DATA_IN register, and do some
+     post-processing *)
+  Local Ltac write_data_in_n n :=
+    eapply interact_write_data_in with (i:=n);
+    [ lazymatch goal with
+      | |- _ = word.add _ _ =>
+        subst_lets; simplify_implicits;
+        cbn [Z.of_nat Pos.of_succ_nat Pos.succ]; ring
+      | _ => idtac
+      end;
+      try post_interaction ..
+    | intros;
+      try lazymatch goal with
+          | H : write_step _ _ _ _ |- _ =>
+            cbv [write_step] in H;
+            rewrite data_in_from_index_category in H by lia; subst
+          end
+    ].
+
+  (* same as write_data_in_n but with extra processing to prove we didn't
+     transition to the BUSY state after the write because there are still
+     unwritten input registers *)
+  Local Ltac write_data_in_nonlast_n n :=
+    write_data_in_n n;
+    [ ..
+    | lazymatch goal with
+      | H : context [match get_aes_input ?d with _ => _ end] |- _ =>
+        cbn [data_in_from_index nth] in H;
+        rewrite get_aes_input_none in H
+          by (cbv [write_input_reg];
+              repeat match goal with H : ?x = None |- _ => rewrite H end;
+              tauto)
+      end
+    ].
+
+  (* apply interact_read_data_out for the nth DATA_OUT register, and do some
+     post-processing *)
+  Local Ltac read_data_out_n n :=
+    eapply interact_read_data_out with (i:=n);
+    [lazymatch goal with
+      | |- _ = word.add _ _ =>
+        subst_lets; simplify_implicits;
+        cbn [Z.of_nat Pos.of_succ_nat Pos.succ]; ring
+      | _ => idtac
+      end;
+      try post_interaction ..
+    | intros;
+      try lazymatch goal with
+          | H : read_step _ _ _ _ |- _ =>
+            cbv [read_step] in H;
+            rewrite data_out_from_index_category in H by lia;
+            cbn [read_step read_output_reg data_out_from_index nth] in H;
+            cbn [done_data_out0 done_data_out1 done_data_out2 done_data_out3] in H;
+            destruct H as [? [H ?]];
+            inversion H; clear H; subst
+          end
+    ];
+    (* try eauto on leftover side condtions now that evars have been filled
+       in *)
+    [
+      cbn [data_out_from_index nth done_data_out0 done_data_out1
+                               done_data_out2 done_data_out3];
+      eauto .. | ].
 
   Local Notation aes_op_t := (enum_member aes_op) (only parsing).
   Local Notation aes_mode_t := (enum_member aes_mode) (only parsing).
@@ -371,10 +552,11 @@ Section Proofs.
         call function_env aes_data_ready tr m (aes_globals ++ args)
              (fun tr' m' rets =>
                 exists (status out : Semantics.word) (s' : state),
-                  (* trace has exactly one new read value *)
-                  tr' = (map.empty, READ, [AES_STATUS],(map.empty,[status])) :: tr
-                  (* ...and there is a new state matching the new trace *)
-                  /\ execution tr' s'
+                  (* the new state matches the new trace *)
+                  execution tr' s'
+                  (* ...and there exists a single valid status-read step between
+                     the old and new state, and the read result was [status] *)
+                  /\ read_step s STATUS status s'
                   (* ...and all the same properties as before hold on the memory *)
                   /\ R m'
                   (* ...and there is one output value *)
@@ -390,8 +572,7 @@ Section Proofs.
     (* initial processing *)
     repeat straightline.
 
-    (* read STATUS *)
-    interaction_with_reg STATUS.
+    read_status.
     repeat straightline.
 
     (* done; prove postcondition *)
@@ -411,10 +592,11 @@ Section Proofs.
         call function_env aes_data_valid tr m (aes_globals ++ args)
              (fun tr' m' rets =>
                 exists (status out : Semantics.word) (s' : state),
-                  (* trace has exactly one new read value *)
-                  tr' = (map.empty, READ, [AES_STATUS],(map.empty,[status])) :: tr
-                  (* ...and there is a new state matching the new trace *)
-                  /\ execution tr' s'
+                  (* the new state matches the new trace *)
+                  execution tr' s'
+                  (* ...and there exists a single valid status-read step between
+                     the old and new state, and the read result was [status] *)
+                  /\ read_step s STATUS status s'
                   (* ...and all the same properties as before hold on the memory *)
                   /\ R m'
                   (* ...and there is one output value *)
@@ -431,8 +613,7 @@ Section Proofs.
     (* initial processing *)
     repeat straightline.
 
-    (* read STATUS *)
-    interaction_with_reg STATUS.
+    read_status.
     repeat straightline.
 
     (* done; prove postcondition *)
@@ -452,10 +633,11 @@ Section Proofs.
         call function_env aes_idle tr m (aes_globals ++ args)
              (fun tr' m' rets =>
                 exists (status out : Semantics.word) (s' : state),
-                  (* trace has exactly one new read value *)
-                  tr' = (map.empty, READ, [AES_STATUS],(map.empty,[status])) :: tr
-                  (* ...and there is a new state matching the new trace *)
-                  /\ execution tr' s'
+                  (* the new state matches the new trace *)
+                  execution tr' s'
+                  (* ...and there exists a single valid status-read step between
+                     the old and new state, and the read result was [status] *)
+                  /\ read_step s STATUS status s'
                   (* ...and all the same properties as before hold on the memory *)
                   /\ R m'
                   (* ...and there is one output value *)
@@ -472,8 +654,7 @@ Section Proofs.
     (* initial processing *)
     repeat straightline.
 
-    (* read STATUS *)
-    interaction_with_reg STATUS.
+    read_status.
     repeat straightline.
 
     (* done; prove postcondition *)
@@ -506,8 +687,10 @@ Section Proofs.
                 (* the circuit is in IDLE state with the correct control
                    register value and no other known register values *)
                 (exists ctrl,
-                    execution tr' (IDLE (map.put (map:=parameters.regs)
-                                                 map.empty AES_CTRL ctrl))
+                    execution tr' (IDLE (Build_idle_data ctrl None None None None
+                                                           None None None None
+                                                           None None None None
+                                                           None None None None))
                     /\ ctrl_operation ctrl = negb (word.eqb aes_cfg_operation (word.of_Z 0))
                     /\ ctrl_mode ctrl = aes_cfg_mode
                     /\ ctrl_key_len ctrl = aes_cfg_key_len
@@ -525,9 +708,11 @@ Section Proofs.
     (* initial processing *)
     repeat straightline.
 
-    (* write CTRL *)
-    interaction_with_reg CTRL.
+    write_control; [ cbn iota; trivial | ].
     repeat straightline.
+
+    (* simplify post-write guarantees *)
+    cbn [write_step reg_category] in *.
 
     (* done; prove postcondition *)
     ssplit; auto; [ ].
@@ -546,16 +731,12 @@ Section Proofs.
                pose proof has_size_nonneg _ _ H
            end.
 
-    (* infer information from the last step *)
-    cbn [parameters.write_step state_machine_parameters] in *.
-    infer; subst.
-
     simplify_implicits.
 
     (* split cases *)
     eexists; ssplit.
     { (* prove that the execution trace is OK *)
-      eassumption. }
+      subst; eassumption. }
     { (* prove that the "operation" flag is correct *)
       cbv [ctrl_operation].
       rewrite !is_flag_set_or_shiftl_low by lia.
@@ -576,8 +757,7 @@ Section Proofs.
 
   Global Instance spec_of_aes_key_put : spec_of aes_key_put :=
     fun function_env =>
-      forall (tr : trace) (m : mem) R
-        (rs : known_register_state)
+      forall (tr : trace) (m : mem) R (data : idle_data)
         (key_len key_arr_ptr : Semantics.word) (key_arr : list Semantics.word),
         (* key_len is a member of the aes_key_len enum *)
         aes_key_len_t key_len ->
@@ -588,53 +768,20 @@ Section Proofs.
                            then 4%nat else if word.eqb key_len kAes192
                                        then 6%nat else 8%nat) ->
         (* circuit must be in IDLE state *)
-        execution tr (IDLE rs) ->
+        execution tr (IDLE data) ->
         let args := [key_arr_ptr; key_len] in
         call function_env aes_key_put tr m (aes_globals ++ args)
              (fun tr' m' rets =>
                 (* the circuit is in IDLE state with the key registers updated *)
-                (exists rs',
-                    map.putmany_of_list_zip
-                      [reg_addr KEY0; reg_addr KEY1; reg_addr KEY2; reg_addr KEY3;
-                      reg_addr KEY4; reg_addr KEY5; reg_addr KEY6; reg_addr KEY7]
-                      (key_arr ++ repeat (word.of_Z 0) (8 - length key_arr)) rs
-                    = Some rs'
-                    /\ execution tr' (IDLE rs'))
+                execution tr'
+                          (IDLE (fold_left
+                                   (fun data i =>
+                                      write_input_reg (key_from_index i) data (nth i key_arr (word.of_Z 0)))
+                                   (seq 0 8) data))
                 (* ...and the same properties as before hold on the memory *)
                 /\ (array scalar32 (word.of_Z 4) key_arr_ptr key_arr * R)%sep m'
                 (* ...and there is no output *)
                 /\ rets = []).
-
-  Local Ltac dexpr_hammer :=
-    subst_lets; simplify_implicits;
-    repeat first [ progress push_unsigned
-                 | rewrite word.unsigned_of_Z in *
-                 | rewrite word.wrap_small in * by lia
-                 | destruct_one_match
-                 | lia ].
-
-  (* TODO: move *)
-  Lemma map_putmany_of_list_zip_snoc {key value} {map : map.map key value}
-        ks vs k v m m' :
-    map.putmany_of_list_zip (map:=map) ks vs m = Some m' ->
-    map.putmany_of_list_zip (ks ++ [k]) (vs ++ [v]) m = Some (map.put m' k v).
-  Proof.
-    revert vs k v m m'; induction ks; destruct vs;
-      [ cbn; congruence | discriminate | discriminate | ].
-    intros. rewrite <-!app_comm_cons. cbn [map.putmany_of_list_zip].
-    auto.
-  Qed.
-
-  (* TODO: move *)
-  Lemma nth_firstn {A} (l : list A) i n d :
-    (i < n)%nat -> nth i (firstn n l) d = nth i l d.
-  Proof.
-    revert l i d. induction n; [ lia | ].
-    destruct l; [ reflexivity | ].
-    destruct i; [ reflexivity | ].
-    cbn [firstn nth]; intros.
-    apply IHn. lia.
-  Qed.
 
   Lemma aes_key_put_correct :
     program_logic_goal_for_function! aes_key_put.
@@ -663,52 +810,6 @@ Section Proofs.
     assert (4 <= length key_arr <= 8)%nat.
     { lazymatch goal with H : length key_arr = _ |- _ => rewrite H end.
       repeat destruct_one_match; lia. }
-
-    (* helper assertion indicating that MMIO addresses in the range we access
-       here are all for key registers *)
-    assert (forall i r,
-               parameters.reg_addr r
-               = word.add AES_KEY0
-                          (word.mul (word.of_Z (Z.of_nat i)) (word.of_Z 4)) ->
-               (i < 8)%nat ->
-               reg_category r = KeyReg)
-      as HKeyReg.
-    { intros i; intros.
-      let H := fresh in
-      assert (i = 0 \/ i = 1 \/ i = 2 \/ i = 3 \/ i = 4 \/ i = 5 \/ i = 6 \/ i = 7)%nat
-        as H by lia;
-        repeat match type of H with _ \/ _ => destruct H as [H | H]; subst end.
-      all:lazymatch goal with
-          | H : parameters.reg_addr _ = ?addr |- _ =>
-            ring_simplify addr in H;
-              first [ apply (reg_addr_unique _ KEY0) in H
-                    | apply (reg_addr_unique _ KEY1) in H
-                    | apply (reg_addr_unique _ KEY2) in H
-                    | apply (reg_addr_unique _ KEY3) in H
-                    | apply (reg_addr_unique _ KEY4) in H
-                    | apply (reg_addr_unique _ KEY5) in H
-                    | apply (reg_addr_unique _ KEY6) in H
-                    | apply (reg_addr_unique _ KEY7) in H ]
-          end.
-      all:subst; reflexivity. }
-
-    (* helper assertion for indexing into list of addresses *)
-    assert (forall i d,
-               (i < 8)%nat ->
-               nth i
-                   [reg_addr KEY0; reg_addr KEY1; reg_addr KEY2;
-                    reg_addr KEY3; reg_addr KEY4; reg_addr KEY5;
-                    reg_addr KEY6; reg_addr KEY7] d
-               = word.add AES_KEY0
-                          (word.mul (word.of_Z (Z.of_nat i)) (word.of_Z 4)))
-      as Hnth_addrs.
-    { intros i ? ?.
-      let H := fresh in
-      assert (i = 0 \/ i = 1 \/ i = 2 \/ i = 3 \/ i = 4 \/ i = 5 \/ i = 6 \/ i = 7)%nat
-        as H by lia;
-        repeat match type of H with _ \/ _ => destruct H as [H | H] end.
-      all:subst i; cbn [nth reg_addr].
-      all:ring. }
 
     (* setup done; now we can proceed with the program logic *)
 
@@ -749,15 +850,16 @@ Section Proofs.
            (invariant:=
               fun v tr' m' l' =>
                 (* the new state is the old one plus the first i keys *)
-                (exists rs',
-                    map.putmany_of_list_zip
-                      (firstn (length key_arr - v)
-                              [reg_addr KEY0; reg_addr KEY1;
-                               reg_addr KEY2; reg_addr KEY3;
-                               reg_addr KEY4; reg_addr KEY5;
-                               reg_addr KEY6; reg_addr KEY7])
-                      (firstn (length key_arr - v) key_arr) rs = Some rs'
-                    /\ execution (p:=state_machine_parameters) tr' (IDLE rs'))
+                execution
+                  (p:=state_machine_parameters) tr'
+                  (IDLE
+                     (fold_left
+                        (fun data i =>
+                           write_input_reg
+                             (key_from_index i) data
+                             (nth i key_arr (word.of_Z 0)))
+                        (seq 0 (length key_arr - v))
+                        data))
                 (* array accesses in bounds *)
                 /\ (0 < v <= length key_arr)%nat
                 (* locals are unaffected except for i *)
@@ -793,8 +895,7 @@ Section Proofs.
       | |- (_ <= _)%nat => lia
       | _ => idtac
       end.
-      cbn [firstn]. eexists; split; [ reflexivity | ].
-      eassumption. }
+      cbn [firstn fold_left]. eassumption. }
 
     { (* the body of the loop proves the invariant if it continues and the
          postcondition if it breaks *)
@@ -837,16 +938,7 @@ Section Proofs.
       (* now, finally, we can process the loop body *)
 
       (* set key register *)
-      interaction ltac:(solve_dexprs).
-      cbn [parameters.write_step state_machine_parameters] in *.
-      infer.
-      match goal with
-      | H : write_step _ _ _ _ |- _ =>
-        rewrite hd_skipn in H;
-          cbv [write_step] in H;
-          erewrite HKeyReg in H by (eassumption || lia)
-      end.
-      infer.
+      write_key.
 
       (* rest of loop body *)
       repeat straightline.
@@ -895,13 +987,9 @@ Section Proofs.
           replace (length key_arr - (v - 1))%nat
             with (S (length key_arr - v))%nat by lia
         end.
-        rewrite !firstn_succ_snoc with (d:=word.of_Z 0) by length_hammer.
-        eexists; ssplit; [ | eassumption ].
-        rewrite Hnth_addrs by lia.
-        lazymatch goal with
-        | H : parameters.reg_addr ?r = ?addr |- context [?addr] =>
-          rewrite <-H end.
-        auto using map_putmany_of_list_zip_snoc. }
+        autorewrite with pull_snoc natsimpl.
+        rewrite <-!hd_skipn.
+        eassumption. }
 
       { (* "break" case; prove postcondition holds after the rest of the function *)
 
@@ -926,16 +1014,16 @@ Section Proofs.
         (* invariant *)
         exists (fun v tr' m' l' =>
              (* the new state is the old one plus the first i keys *)
-             (exists rs',
-                 map.putmany_of_list_zip
-                   (firstn (8 - v)
-                           [reg_addr KEY0; reg_addr KEY1;
-                            reg_addr KEY2; reg_addr KEY3;
-                            reg_addr KEY4; reg_addr KEY5;
-                            reg_addr KEY6; reg_addr KEY7])
-                   (key_arr ++ repeat (word.of_Z 0) (8 - v - length key_arr))
-                   rs = Some rs'
-                 /\ execution (p:=state_machine_parameters) tr' (IDLE rs'))
+             execution
+               (p:=state_machine_parameters) tr'
+               (IDLE
+                  (fold_left
+                     (fun data i =>
+                        write_input_reg
+                          (key_from_index i) data
+                          (nth i key_arr (word.of_Z 0)))
+                     (seq 0 (8 - v))
+                     data))
              (* bounds for # iterations *)
              /\ (v <= 8 - length key_arr)%nat
              (* locals are unaffected except for i *)
@@ -947,7 +1035,8 @@ Section Proofs.
         { (* invariant holds at loop start *)
           exists (8 - length key_arr)%nat. (* total # iterations *)
           replace (8 - (8 - length key_arr))%nat with (length key_arr) by lia.
-          rewrite Nat.sub_diag. cbn [repeat]. rewrite app_nil_r.
+          (*
+          rewrite Nat.sub_diag. cbn [repeat]. rewrite app_nil_r.*)
           ssplit;
           lazymatch goal with
             | |- ?m = map.put ?m _ _ =>
@@ -958,26 +1047,14 @@ Section Proofs.
             | _ => idtac
           end.
 
-          eexists; ssplit; [ | eassumption ].
-
-          (* rewrite postcondition to be firstn ++ last *)
           lazymatch goal with
-          | H : map.putmany_of_list_zip (firstn ?n _) (firstn ?n ?vs) _ = Some _
-            |- context [map.putmany_of_list_zip ?ks ?vs ?m] =>
-            replace (map.putmany_of_list_zip ks vs m)
-              with (map.putmany_of_list_zip
-                      (firstn (S n) ks) (firstn (S n) vs) m)
-              by (rewrite !firstn_all2 by length_hammer;
-                  f_equal; apply firstn_all2; lia);
-              rewrite !firstn_succ_snoc with (d:=word.of_Z 0) by length_hammer
+          | H : context [write_input_reg _ (fold_left _ (seq 0 ?n) _)]
+            |- context [fold_left _ (seq 0 ?m)] =>
+            replace (seq 0 m) with (seq 0 (S n)) by (f_equal; lia)
           end.
-          rewrite firstn_firstn, Nat.min_l, nth_firstn by lia.
-          erewrite map_putmany_of_list_zip_snoc by eassumption.
-          rewrite Hnth_addrs by lia.
-          lazymatch goal with
-          | H : parameters.reg_addr ?r = ?addr |- context [?addr] =>
-            rewrite <-H end.
-          reflexivity. }
+          autorewrite with pull_snoc natsimpl.
+          rewrite <-!hd_skipn.
+          eassumption. }
 
         { (* the body of the loop proves the invariant if it continues and the
              postcondition if it breaks *)
@@ -999,16 +1076,7 @@ Section Proofs.
             repeat straightline.
 
             (* set key register *)
-            interaction ltac:(solve_dexprs).
-            cbn [parameters.write_step state_machine_parameters] in *.
-            infer.
-            match goal with
-            | H : write_step _ _ _ _ |- _ =>
-              cbv [write_step] in H;
-                erewrite HKeyReg in H
-                by (eassumption || lia)
-            end.
-            infer. subst.
+            write_key.
 
           (* rest of loop body *)
           repeat straightline.
@@ -1033,9 +1101,7 @@ Section Proofs.
                 f_equal; apply word.unsigned_inj;
                   subst_lets; push_unsigned; lia
             | |- sep _ _ _ => ecancel_assumption
-            | |- (_ < _)%nat => lia
-            | |- (_ <= _)%nat => lia
-            | _ => idtac
+            | |- ?G => tryif is_lia G then lia else idtac
             end.
 
           (* final invariant case: new register state *)
@@ -1046,20 +1112,13 @@ Section Proofs.
             replace (8 - (v - 1))%nat
               with (S (8 - v))%nat by lia
           end.
-          rewrite (Nat.sub_succ_l (length key_arr) (8 - _)%nat) by lia.
 
           (* list simplifications *)
-          cbn [repeat]. rewrite repeat_cons, app_assoc.
-          rewrite !firstn_succ_snoc with (d:=word.of_Z 0) by length_hammer.
+          autorewrite with pull_snoc natsimpl.
+          autorewrite with push_nth.
 
           (* solve *)
-          simplify_implicits.
-          eexists; ssplit; [ | eassumption ].
-          rewrite Hnth_addrs by lia.
-          lazymatch goal with
-          | H : parameters.reg_addr ?r = ?addr |- context [?addr] =>
-            rewrite <-H end.
-          auto using map_putmany_of_list_zip_snoc. }
+          eassumption. }
 
           { (* post-loop; given invariant and loop-break condition, prove
                postcondition holds after the rest of the function *)
@@ -1077,38 +1136,36 @@ Section Proofs.
             end.
 
             eexists; ssplit; eauto; [ ].
-            eexists; ssplit; eauto; [ ].
+
             lazymatch goal with
-            | H : map.putmany_of_list_zip ?ks1 ?vs1 ?m = Some ?m'
-              |- map.putmany_of_list_zip ?ks2 ?vs2 ?m = Some ?m' =>
-              replace ks2 with ks1;
-                [ replace vs2 with vs1; [ exact H | ] | ]
+            | H : context [fold_left _ (seq 0 (8 - ?v))] |- _ =>
+              replace (8 - v)%nat with 8%nat in H by lia
             end.
-            { repeat (f_equal; try lia). }
-            { apply firstn_all2. length_hammer. } } } } }
+            eassumption. } } } }
   Qed.
 
   Global Instance spec_of_aes_iv_put : spec_of aes_iv_put :=
     fun function_env =>
-      forall (tr : trace) (m : mem) R
-        (rs : known_register_state)
-        (iv_ptr iv0 iv1 iv2 iv3 : Semantics.word),
+      forall (tr : trace) (m : mem) R (data : idle_data)
+        (iv_ptr : Semantics.word) (iv_arr : list Semantics.word),
         (* iv array is in memory *)
-        (array scalar32 (word.of_Z 4) iv_ptr [iv0;iv1;iv2;iv3] * R)%sep m ->
+        (array scalar32 (word.of_Z 4) iv_ptr iv_arr * R)%sep m ->
+        (* iv array has 4 elements *)
+        length iv_arr = 4%nat ->
         (* circuit must be in IDLE state *)
-        execution tr (IDLE rs) ->
+        execution tr (IDLE data) ->
         let args := [iv_ptr] in
         call function_env aes_iv_put tr m (aes_globals ++ args)
              (fun tr' m' rets =>
                 (* the circuit is in IDLE state with the iv registers updated *)
                 execution tr'
-                          (IDLE (map.putmany_of_list
-                                   [(reg_addr IV0, iv0)
-                                    ; (reg_addr IV1, iv1)
-                                    ; (reg_addr IV2, iv2)
-                                    ; (reg_addr IV3, iv3)] rs))
+                          (IDLE (fold_left
+                                   (fun data i =>
+                                      write_input_reg (iv_from_index i) data
+                                                      (nth i iv_arr (word.of_Z 0)))
+                                   (seq 0 4) data))
                 (* ...and the same properties as before hold on the memory *)
-                /\ (array scalar32 (word.of_Z 4) iv_ptr [iv0;iv1;iv2;iv3] * R)%sep m'
+                /\ (array scalar32 (word.of_Z 4) iv_ptr iv_arr * R)%sep m'
                 (* ...and there is no output *)
                 /\ rets = []).
 
@@ -1120,6 +1177,7 @@ Section Proofs.
     simplify_implicits.
 
     (* simplify array predicate *)
+    destruct_lists_by_length.
     cbn [array] in *.
     repeat match goal with
            | H : context [scalar32 ?addr] |- _ =>
@@ -1138,22 +1196,21 @@ Section Proofs.
 
     (* i = 0 *)
     split; repeat straightline; [ dexpr_hammer | ].
-    interaction_with_reg IV0. infer; subst.
-    repeat straightline.
+    write_iv_n 0%nat. repeat straightline.
 
     (* i = 1 *)
     split; repeat straightline; [ dexpr_hammer | ].
-    interaction_with_reg IV1. infer; subst.
+    write_iv_n 1%nat; [ simplify_implicits; subst_lets; ring | ].
     repeat straightline.
 
     (* i = 2 *)
     split; repeat straightline; [ dexpr_hammer | ].
-    interaction_with_reg IV2. infer; subst.
+    write_iv_n 2%nat; [ simplify_implicits; subst_lets; ring | ].
     repeat straightline.
 
     (* i = 3 *)
     split; repeat straightline; [ dexpr_hammer | ].
-    interaction_with_reg IV3. infer; subst.
+    write_iv_n 3%nat; [ simplify_implicits; subst_lets; ring | ].
     repeat straightline.
 
     (* i = 4; loop done *)
@@ -1170,36 +1227,39 @@ Section Proofs.
 
   Global Instance spec_of_aes_data_put : spec_of aes_data_put :=
     fun function_env =>
-      forall (tr : trace) (m : mem) R
-        (rs : known_register_state)
-        (data_ptr data0 data1 data2 data3 : Semantics.word),
-        (* data array is in memory *)
-        (array scalar32 (word.of_Z 4) data_ptr [data0;data1;data2;data3] * R)%sep m ->
+      forall (tr : trace) (m : mem) R (data : idle_data) all_aes_input
+        (input_ptr : Semantics.word) (input_arr : list Semantics.word),
+        (* input array is in memory *)
+        (array scalar32 (word.of_Z 4) input_ptr input_arr * R)%sep m ->
+        (* input array has 4 elements *)
+        length input_arr = 4%nat ->
         (* circuit must be in IDLE state *)
-        execution tr (IDLE rs) ->
-        (* the key and iv registers must be populated *)
-        nregs_populated rs KeyReg = 8%nat ->
-        nregs_populated rs IVReg = 4%nat ->
-        (* the data registers must *not* be populated *)
-        nregs_populated rs DataInReg = 0%nat ->
-        let args := [data_ptr] in
+        execution tr (IDLE data) ->
+        (* input-data registers must not be currently set *)
+        data.(idle_data_in0) = None ->
+        data.(idle_data_in1) = None ->
+        data.(idle_data_in2) = None ->
+        data.(idle_data_in3) = None ->
+        (* adding input-data registers must result in a full set of data
+           (i.e. key and iv registers are already set) *)
+        get_aes_input
+          (fold_left
+             (fun data i =>
+                write_input_reg (data_in_from_index i) data
+                                (nth i input_arr (word.of_Z 0)))
+             (seq 0 4) data) = Some all_aes_input ->
+        let args := [input_ptr] in
         call function_env aes_data_put tr m (aes_globals ++ args)
              (fun tr' m' rets =>
-                exists exp_out,
-                  (* the circuit is now in the BUSY state *)
-                  execution tr' (BUSY (unset_inp_regs rs) exp_out
-                                      timing.ndelays_core)
-                  (* ...and the expected output matches the AES spec for this data *)
-                  /\ aes_expected_output
-                      (map.putmany_of_list
-                         [(reg_addr DATA_IN0, data0)
-                          ; (reg_addr DATA_IN1, data1)
-                          ; (reg_addr DATA_IN2, data2)
-                          ; (reg_addr DATA_IN3, data3)] rs) = Some exp_out
-                  (* ...and the same properties as before hold on the memory *)
-                  /\ (array scalar32 (word.of_Z 4) data_ptr [data0;data1;data2;data3] * R)%sep m'
-                  (* ...and there is no output *)
-                  /\ rets = []).
+                (* the circuit is now in the BUSY state *)
+                execution tr' (BUSY (Build_busy_data
+                                       (idle_ctrl data)
+                                       (aes_expected_output all_aes_input)
+                                       timing.ndelays_core))
+                (* ...and the same properties as before hold on the memory *)
+                /\ (array scalar32 (word.of_Z 4) input_ptr input_arr * R)%sep m'
+                (* ...and there is no output *)
+                /\ rets = []).
 
   Lemma aes_data_put_correct :
     program_logic_goal_for_function! aes_data_put.
@@ -1209,6 +1269,7 @@ Section Proofs.
     simplify_implicits.
 
     (* simplify array predicate *)
+    destruct_lists_by_length.
     cbn [array] in *.
     repeat match goal with
            | H : context [scalar32 ?addr] |- _ =>
@@ -1227,28 +1288,25 @@ Section Proofs.
 
     (* i = 0 *)
     split; repeat straightline; [ dexpr_hammer | ].
-    interaction_with_reg DATA_IN0.
-    infer; subst; clear_old_executions.
-    repeat straightline.
-
+    write_data_in_nonlast_n 0%nat. repeat straightline.
 
     (* i = 1 *)
     split; repeat straightline; [ dexpr_hammer | ].
-    interaction_with_reg DATA_IN1.
-    infer; subst; clear_old_executions.
-    repeat straightline.
+    write_data_in_nonlast_n 1%nat. repeat straightline.
 
     (* i = 2 *)
     split; repeat straightline; [ dexpr_hammer | ].
-    interaction_with_reg DATA_IN2.
-    infer; subst; clear_old_executions.
-    repeat straightline.
+    write_data_in_nonlast_n 2%nat. repeat straightline.
 
     (* i = 3 *)
     split; repeat straightline; [ dexpr_hammer | ].
-    interaction_with_reg DATA_IN3.
-    infer; subst; clear_old_executions.
-    repeat straightline.
+    write_data_in_n 3%nat. repeat straightline.
+    lazymatch goal with
+    | H1 : get_aes_input (fold_left _ _ _) = Some _,
+      H2 : context [match get_aes_input _ with _ => _ end] |- _ =>
+      cbn [fold_left seq nth data_in_from_index] in H1, H2;
+        rewrite H1 in H2
+    end.
 
     (* i = 4; loop done *)
     ssplit; repeat straightline; [ dexpr_hammer | ].
@@ -1260,13 +1318,7 @@ Section Proofs.
              progress ring_simplify addr
            end.
 
-    eexists; ssplit; eauto; [ ].
-    (* find and apply execution hypothesis by asserting states are equal *)
-    lazymatch goal with H : execution ?t ?s1 |- execution ?t ?s2 =>
-                        let H' := fresh in
-                        assert (s2 = s1) as H'; [ | rewrite H'; apply H ]
-    end.
-    rewrite !unset_inp_regs_put. reflexivity.
+    ssplit; eauto.
   Qed.
 
   (* TODO: the real state machine is slightly more complex; AES block can get
@@ -1275,36 +1327,39 @@ Section Proofs.
      exactly the same as aes_data_put. *)
   Global Instance spec_of_aes_data_put_wait : spec_of aes_data_put_wait :=
     fun function_env =>
-      forall (tr : trace) (m : mem) R
-        (rs : known_register_state)
-        (data_ptr data0 data1 data2 data3 : Semantics.word),
-        (* data array is in memory *)
-        (array scalar32 (word.of_Z 4) data_ptr [data0;data1;data2;data3] * R)%sep m ->
+      forall (tr : trace) (m : mem) R (data : idle_data) all_aes_input
+        (input_ptr : Semantics.word) (input_arr : list Semantics.word),
+        (* input array is in memory *)
+        (array scalar32 (word.of_Z 4) input_ptr input_arr * R)%sep m ->
+        (* input array has 4 elements *)
+        length input_arr = 4%nat ->
         (* circuit must be in IDLE state *)
-        execution tr (IDLE rs) ->
-        (* the key and iv registers must be populated *)
-        nregs_populated rs KeyReg = 8%nat ->
-        nregs_populated rs IVReg = 4%nat ->
-        (* the data registers must *not* be populated *)
-        nregs_populated rs DataInReg = 0%nat ->
-        let args := [data_ptr] in
+        execution tr (IDLE data) ->
+        (* input-data registers must not be currently set *)
+        data.(idle_data_in0) = None ->
+        data.(idle_data_in1) = None ->
+        data.(idle_data_in2) = None ->
+        data.(idle_data_in3) = None ->
+        (* adding input-data registers must result in a full set of data
+           (i.e. key and iv registers are already set) *)
+        get_aes_input
+          (fold_left
+             (fun data i =>
+                write_input_reg (data_in_from_index i) data
+                                (nth i input_arr (word.of_Z 0)))
+             (seq 0 4) data) = Some all_aes_input ->
+        let args := [input_ptr] in
         call function_env aes_data_put_wait tr m (aes_globals ++ args)
              (fun tr' m' rets =>
-                exists exp_out,
-                  (* the circuit is now in the BUSY state *)
-                  execution tr' (BUSY (unset_inp_regs rs) exp_out
-                                      timing.ndelays_core)
-                  (* ...and the expected output matches the AES spec for this data *)
-                  /\ aes_expected_output
-                      (map.putmany_of_list
-                         [(reg_addr DATA_IN0, data0)
-                          ; (reg_addr DATA_IN1, data1)
-                          ; (reg_addr DATA_IN2, data2)
-                          ; (reg_addr DATA_IN3, data3)] rs) = Some exp_out
-                  (* ...and the same properties as before hold on the memory *)
-                  /\ (array scalar32 (word.of_Z 4) data_ptr [data0;data1;data2;data3] * R)%sep m'
-                  (* ...and there is no output *)
-                  /\ rets = []).
+                (* the circuit is now in the BUSY state *)
+                execution tr' (BUSY (Build_busy_data
+                                       (idle_ctrl data)
+                                       (aes_expected_output all_aes_input)
+                                       timing.ndelays_core))
+                (* ...and the same properties as before hold on the memory *)
+                /\ (array scalar32 (word.of_Z 4) input_ptr input_arr * R)%sep m'
+                (* ...and there is no output *)
+                /\ rets = []).
 
   Lemma aes_data_put_wait_correct :
     program_logic_goal_for_function! aes_data_put_wait.
@@ -1324,30 +1379,19 @@ Section Proofs.
 
     (* simplify guarantees *)
     logical_simplify; subst.
-    lazymatch goal with
-    | H : execution (_ :: _) _ |- _ =>
-      pose proof H; apply invert1_execution in H; logical_simplify
-    end.
-    invert_step; subst.
-    cbn [parameters.reg_addr parameters.write_step parameters.read_step
-                             state_machine_parameters] in *.
-    infer; subst.
-    (* assert that the register address we just read is STATUS *)
-    lazymatch goal with
-    | H : reg_addr ?r = AES_STATUS |- _ =>
-      apply (reg_addr_unique r STATUS) in H; subst
-    end.
-    cbv [status_matches_state] in *. simplify_implicits.
+    cbn [read_step reg_category] in *.
+    cbv [status_matches_state] in *.
+    logical_simplify; simplify_implicits.
     repeat match goal with
            | H : (_ && _)%bool = true |- _ => apply Bool.andb_true_iff in H; destruct H
            | H : word.eqb _ _ = _ |- _ => apply word.eqb_false in H
            | H : is_flag_set _ _  = _ |- _ => progress rewrite H in *
            end.
+    subst.
 
     (* loop done *)
     repeat straightline.
-    split; repeat straightline; [ dexpr_hammer; try congruence; reflexivity | ].
-    split; repeat straightline; [ dexpr_hammer | ].
+    split; repeat straightline; [ dexpr_hammer; congruence | ].
 
     (* call aes_data_put *)
     straightline_call; eauto; [ ].
@@ -1361,36 +1405,31 @@ Section Proofs.
 
   Global Instance spec_of_aes_data_get : spec_of aes_data_get :=
     fun function_env =>
-      forall (tr : trace) (m : mem) R
-        (rs : known_register_state)
-        (data_ptr data0 data1 data2 data3 : Semantics.word),
-        (* data array is in memory, with arbitrary values *)
-        (array scalar32 (word.of_Z 4) data_ptr [data0;data1;data2;data3] * R)%sep m ->
+      forall (tr : trace) (m : mem) R (data : done_data)
+        (data_ptr out0 out1 out2 out3 : Semantics.word)
+        (data_arr : list Semantics.word),
+        (* data array is in memory, with arbitrary initital values *)
+        (array scalar32 (word.of_Z 4) data_ptr data_arr * R)%sep m ->
+        length data_arr = 4%nat ->
         (* circuit must be in the DONE state *)
-        execution tr (DONE rs) ->
-        (* the output data registers must be populated *)
-        nregs_populated rs DataOutReg = 4%nat ->
+        execution tr (DONE data) ->
+        (* the output registers must all be populated *)
+        data.(done_data_out0) = Some out0 ->
+        data.(done_data_out1) = Some out1 ->
+        data.(done_data_out2) = Some out2 ->
+        data.(done_data_out3) = Some out3 ->
         let args := [data_ptr] in
         call function_env aes_data_get tr m (aes_globals ++ args)
              (fun tr' m' rets =>
-                exists out0 out1 out2 out3,
-                  (* the circuit is now in the IDLE state with output registers unset *)
-                  execution tr' (IDLE (map.remove
-                                         (map.remove
-                                            (map.remove
-                                               (map.remove rs
-                                                           (reg_addr DATA_OUT0))
-                                               (reg_addr DATA_OUT1))
-                                            (reg_addr DATA_OUT2))
-                                         (reg_addr DATA_OUT3)))
-                  (* ...and the array now holds the values from the output registers *)
-                  /\ (array scalar32 (word.of_Z 4) data_ptr [out0;out1;out2;out3] * R)%sep m'
-                  /\ reg_lookup rs DATA_OUT0 = Some out0
-                  /\ reg_lookup rs DATA_OUT1 = Some out1
-                  /\ reg_lookup rs DATA_OUT2 = Some out2
-                  /\ reg_lookup rs DATA_OUT3 = Some out3
-                  (* ...and there are no return values *)
-                  /\ rets = []).
+                (* the circuit is now in the IDLE state with output registers unset *)
+                execution tr' (IDLE (Build_idle_data
+                                       (done_ctrl data) None None None None None None None None
+                                       None None None None None None None None))
+                (* ...and the array now holds the values from the output registers *)
+                /\ (array scalar32 (word.of_Z 4) data_ptr [out0;out1;out2;out3] * R)%sep m'
+                (* ...and there are no return values *)
+                /\ rets = []).
+
 
   Lemma aes_data_get_correct :
     program_logic_goal_for_function! aes_data_get.
@@ -1400,6 +1439,7 @@ Section Proofs.
     simplify_implicits.
 
     (* simplify array predicate *)
+    destruct_lists_by_length.
     cbn [array] in *.
     repeat match goal with
            | H : context [scalar32 ?addr] |- _ =>
@@ -1416,13 +1456,18 @@ Section Proofs.
 
     (* process each iteration of the while loop *)
 
+    destruct data;
+      cbn [AesSemantics.done_ctrl
+             AesSemantics.done_data_out0
+             AesSemantics.done_data_out1
+             AesSemantics.done_data_out2
+             AesSemantics.done_data_out3] in *; subst.
+
     (* i = 0 *)
     split; repeat straightline; [ dexpr_hammer | ].
 
     (* read register *)
-    interaction_with_reg DATA_OUT0.
-    infer; subst; clear_old_executions.
-    repeat straightline.
+    read_data_out_n 0%nat. repeat straightline.
 
     (* store result in memory *)
     simplify_implicits.
@@ -1437,26 +1482,7 @@ Section Proofs.
     split; repeat straightline; [ dexpr_hammer | ].
 
     (* read register *)
-    interaction_with_reg DATA_OUT1.
-    infer; subst; clear_old_executions.
-    repeat straightline.
-
-    (* store result in memory *)
-    simplify_implicits.
-    ring_simplify_store_addr.
-    (* the following line is in [straightline] but needs simplify_implicits for
-       it to work *)
-    eapply store_four_of_sep_32bit;
-      [ reflexivity | simplify_implicits; solve [ ecancel_assumption ] |  ].
-    repeat straightline.
-
-    (* i = 2 *)
-    split; repeat straightline; [ dexpr_hammer | ].
-
-    (* read register *)
-    interaction_with_reg DATA_OUT2.
-    infer; subst; clear_old_executions.
-    repeat straightline.
+    read_data_out_n 1%nat. repeat straightline.
 
     (* store result in memory *)
     simplify_implicits.
@@ -1471,9 +1497,22 @@ Section Proofs.
     split; repeat straightline; [ dexpr_hammer | ].
 
     (* read register *)
-    interaction_with_reg DATA_OUT3.
-    infer; subst; clear_old_executions.
+    read_data_out_n 2%nat. repeat straightline.
+
+    (* store result in memory *)
+    simplify_implicits.
+    ring_simplify_store_addr.
+    (* the following line is in [straightline] but needs simplify_implicits for
+       it to work *)
+    eapply store_four_of_sep_32bit;
+      [ reflexivity | simplify_implicits; solve [ ecancel_assumption ] |  ].
     repeat straightline.
+
+    (* i = 3 *)
+    split; repeat straightline; [ dexpr_hammer | ].
+
+    (* read register *)
+    read_data_out_n 3%nat. repeat straightline.
 
     (* store result in memory *)
     simplify_implicits.
@@ -1494,45 +1533,34 @@ Section Proofs.
              progress ring_simplify addr
            end.
 
-    (* change register lookups to refer to original register state *)
-    repeat lazymatch goal with
-           | H : reg_lookup (map.remove _ _) _ = Some _ |- _ =>
-             cbv [reg_lookup] in H;
-               rewrite !map.get_remove_dec in H;
-               rewrite !word.eqb_ne in H by (apply reg_addr_neq; congruence)
-           end.
-
-    do 4 eexists; ssplit; eauto; [ ].
+    ssplit; eauto; [ ].
     simplify_implicits.
     ecancel_assumption.
   Qed.
 
-  Definition output_matches_state out s :=
+  Definition output_matches_state (out : aes_output) (s : state) : Prop :=
     match s with
-    | DONE rs =>
-      reg_lookup rs DATA_OUT0 = Some out.(data_out0)
-      /\ reg_lookup rs DATA_OUT1 = Some out.(data_out1)
-      /\ reg_lookup rs DATA_OUT2 = Some out.(data_out2)
-      /\ reg_lookup rs DATA_OUT3 = Some out.(data_out3)
-    | BUSY _ exp_output _ => exp_output = out
+    | BUSY data => busy_exp_output data = out
+    | DONE data =>
+      data = done_data_from_output (done_ctrl data) out
     | _ => False
     end.
 
-  Definition get_register_state s : known_register_state :=
+  Definition get_ctrl (s : state) : Semantics.word :=
     match s with
-    | DONE rs => rs
-    | BUSY rs _ _ => rs
-    | IDLE rs => rs
-    | UNINITIALIZED => map.empty
+    | UNINITIALIZED => word.of_Z 0 (* dummy value *)
+    | IDLE data => idle_ctrl data
+    | BUSY data => busy_ctrl data
+    | DONE data => done_ctrl data
     end.
 
   Global Instance spec_of_aes_data_get_wait : spec_of aes_data_get_wait :=
     fun function_env =>
-      forall (tr : trace) (m : mem) R
-        (out : aes_output)
-        (data_ptr data0 data1 data2 data3 : Semantics.word) (s : state),
-        (* data array is in memory, with arbitrary values *)
-        (array scalar32 (word.of_Z 4) data_ptr [data0;data1;data2;data3] * R)%sep m ->
+      forall (tr : trace) (m : mem) R (out : aes_output)
+        (data_ptr : Semantics.word) (data_arr : list Semantics.word) (s : state),
+        (* data array is in memory, with arbitrary initital values *)
+        (array scalar32 (word.of_Z 4) data_ptr data_arr * R)%sep m ->
+        length data_arr = 4%nat ->
         (* circuit must be in the DONE or BUSY state (otherwise we can't prove
            termination) and expected or already-written output matches out *)
         execution tr s ->
@@ -1541,14 +1569,9 @@ Section Proofs.
         call function_env aes_data_get_wait tr m (aes_globals ++ args)
              (fun tr' m' rets =>
                 (* the circuit is now in the IDLE state with output registers unset *)
-                execution tr' (IDLE (map.remove
-                                       (map.remove
-                                          (map.remove
-                                             (map.remove (get_register_state s)
-                                                         (reg_addr DATA_OUT0))
-                                             (reg_addr DATA_OUT1))
-                                          (reg_addr DATA_OUT2))
-                                       (reg_addr DATA_OUT3)))
+                execution tr' (IDLE (Build_idle_data (get_ctrl s) None None None None
+                                                     None None None None None None None None
+                                                     None None None None))
                 (* ...and the array now holds the values from the expected output *)
                 /\ (array scalar32 (word.of_Z 4) data_ptr
                          [out.(data_out0)
@@ -1558,110 +1581,6 @@ Section Proofs.
                 (* ...and there are no return values *)
                 /\ rets = []).
 
-  Lemma unset_inp_regs_ignores_outregs rs out :
-    aes_expected_output rs = Some out ->
-    nregs_populated (unset_inp_regs rs) DataOutReg = nregs_populated rs DataOutReg.
-  Proof.
-    cbv [unset_inp_regs]. cbv [aes_expected_output option_bind].
-    repeat (destruct_one_match; try congruence); [ ]. intros.
-    repeat (erewrite nregs_populated_remove
-             by (cbv [reg_lookup];
-                 rewrite ?map.get_remove_diff by (apply reg_addr_neq; congruence);
-                 eassumption);
-            cbn [reg_category reg_category_eqb]).
-    reflexivity.
-  Qed.
-
-  Lemma map_remove_put_same m k v :
-    map.remove (map:=parameters.regs) (map.put m k v) k = map.remove m k.
-  Proof.
-    apply map.map_ext; intros.
-    rewrite ?map.get_remove_dec, ?map.get_put_dec;
-      destruct_one_match; subst; reflexivity.
-  Qed.
-
-  Lemma map_remove_put_diff m k1 k2 v :
-    k1 <> k2 ->
-    map.remove (map:=parameters.regs) (map.put m k1 v) k2 = map.put (map.remove m k2) k1 v.
-  Proof.
-    intros. apply map.map_ext; intros.
-    rewrite ?map.get_remove_dec, ?map.get_put_dec, ?map.get_remove_dec;
-      repeat destruct_one_match; subst; congruence.
-  Qed.
-
-  (* if a put causes more registers to be populated, then the put must set a
-     register that was not previously set *)
-  Lemma nregs_populated_increase rs r v c :
-    (nregs_populated rs c
-     < nregs_populated (map.put rs (reg_addr r) v) c)%nat ->
-    reg_lookup rs r = None.
-  Proof.
-    cbv [nregs_populated reg_lookup]. intros.
-    destr (map.get rs (reg_addr r)); [ exfalso | reflexivity ].
-    erewrite map.fold_remove with (m:=rs) (k:=reg_addr r) in H;
-      [ | intros; repeat destruct_one_match; reflexivity | eassumption ].
-    erewrite map.fold_remove
-      with (m:=map.put rs _ _) (k:=reg_addr r) in H;
-      [ | intros; repeat destruct_one_match; reflexivity
-        | apply map.get_put_same ].
-    rewrite map_remove_put_same in *.
-    destruct_one_match_hyp; lia.
-  Qed.
-
-  Lemma nregs_populated_set_out_regs rs out :
-    nregs_populated (set_out_regs rs out) DataOutReg = 4%nat.
-  Proof.
-    cbv [set_out_regs nregs_populated].
-    repeat match goal with
-           | |- context [map.put _ ?key] =>
-             erewrite map.fold_remove with (k:=key);
-               [ | intros; repeat destruct_one_match; reflexivity
-                 | rewrite ?map.get_remove_diff, ?map.get_put_diff
-                   by (apply reg_addr_neq; congruence);
-                   apply map.get_put_same ];
-               rewrite addr_in_category_reg_addr; cbn [reg_category reg_category_eqb];
-                 rewrite ?map_remove_put_diff by (apply reg_addr_neq; congruence);
-                 rewrite map_remove_put_same
-           end.
-    repeat apply (f_equal S).
-    lazymatch goal with
-    | |- map.fold ?f ?r0 ?m = _ =>
-      let H' := fresh in
-      pose proof map.fold_to_list f r0 m as H';
-        destruct H' as [l [Heq Hin] ]; rewrite Heq;
-          rewrite <-(rev_involutive l)
-    end.
-    rewrite fold_left_rev_right.
-    eapply fold_left_invariant with (I:= eq 0%nat); auto; [ ].
-    intros. destruct_products; subst.
-    repeat lazymatch goal with
-           | H : In _ (rev _) |- _ => rewrite <-in_rev in H
-           | H : In (?k,?v) ?l |- _ => apply Hin in H
-           | H : context [map.get (map.remove _ _)] |- _ =>
-             rewrite map.get_remove_dec in H
-           end.
-    repeat (destruct_one_match_hyp; try congruence).
-    cbv [addr_in_category].
-    cbn [all_regs existsb reg_category reg_category_eqb].
-    boolsimpl. destruct_one_match; try reflexivity; [ ].
-    repeat lazymatch goal with
-           | H : (_ || _)%bool = true |- _ => apply Bool.orb_true_iff in H; destruct H
-           | H : word.eqb _ _ = true |- _ => apply word.eqb_true in H
-           | _ => congruence
-           end.
-  Qed.
-
-  Lemma output_matches_state_set_out_regs rs out :
-    output_matches_state out (DONE rs) ->
-    set_out_regs rs out = rs.
-  Proof.
-    cbv [output_matches_state reg_lookup].
-    intros; logical_simplify.
-    cbv [set_out_regs]. apply map.map_ext; intros.
-    rewrite !map.get_put_dec.
-    repeat destruct_one_match; congruence.
-  Qed.
-
   Lemma aes_data_get_wait_correct :
     program_logic_goal_for_function! aes_data_get_wait.
   Proof.
@@ -1669,68 +1588,179 @@ Section Proofs.
     repeat straightline.
     simplify_implicits.
 
-    set (max_iterations:=fun s : parameters.state =>
-                           match s with
-                           | BUSY _ _ n => n
-                           | DONE _ => 1%nat
-                           | _ => 0%nat
-                           end).
+    (* separate out cases where s is initially BUSY or DONE *)
+    cbv [output_matches_state] in *.
+    destruct s; try contradiction; [ | ].
 
-    (* begin while loop *)
-    let l := lazymatch goal with |- cmd _ _ _ _ ?l _ => l end in
-    apply atleastonce_localsmap
-      with (v0:=max_iterations s)
-           (lt:=lt)
-           (invariant:=
-              fun i tr' m' l' =>
-                exists (s' : parameters.state) is_valid,
-                  (* s' is the state for the new trace *)
-                  execution tr' s'
-                  (* the remaining maximum iterations match the "measure" i *)
-                  /\ max_iterations s' = i
-                  (* as long as the loop continues, we keep setting is_valid to
-                     0, so locals are unchanged until the loop breaks *)
-                  /\ l' = map.put l "is_valid" is_valid
-                  (* expected output still matches *)
-                  /\ output_matches_state out s'
-                  (* s' is related to s either by decrementing counter or being equal *)
-                  /\ match s with
-                    | BUSY rs out n => exists n', s' = BUSY rs out n'
-                    | DONE rs => s' = s
-                    | _ => False
-                    end
-                  (* memory is unaffected *)
-                  /\ (array scalar32 (word.of_Z 4) data_ptr [data0; data1; data2; data3] ⋆ R)%sep m').
-    { apply lt_wf. }
-
-    { (* case in which the loop breaks immediately (cannot happen) *)
-      repeat straightline.
-      exfalso. (* proof by contradiction *)
-
-      repeat lazymatch goal with
-             | v := word.of_Z 0 |- _ => subst v
-             | br := if word.eqb _ (word.of_Z 0) then _ else _ |- _ => subst br
-             end.
-      rewrite @word.unsigned_eqb in * by typeclasses eauto.
-      autorewrite with push_unsigned in *.
-      destruct_one_match_hyp_of_type bool; congruence. }
-
-    { (* proof that invariant holds at loop start *)
-      do 2 eexists; ssplit;
+    { (* case in which the initial state is BUSY *)
       lazymatch goal with
-      | |- execution _ _ => eassumption
-      | |- (?x <= ?x)%nat => reflexivity
-      | |- ?x = ?x => reflexivity
-      | |- sep _ _ _ => eassumption
-      | |- _ = map.put _ _ _ => symmetry; solve [apply map.put_put_same]
-      | |- output_matches_state _ _ =>
-        cbv [output_matches_state] in *;
-        destruct_one_match; solve [eauto]
-      | _ => idtac
-      end; [ ].
-      destruct_one_match; eauto. }
+        H : execution tr (BUSY data) |- _ =>
+        destruct data as [ctrl exp_output max_cycles];
+          cbn [get_ctrl] in *;
+          cbn [busy_ctrl busy_exp_output busy_max_cycles_until_done] in *
+      end.
+      subst.
 
-    { (* invariant holds through loop (or postcondition holds, if loop breaks) *)
+      (* begin while loop *)
+      let l := lazymatch goal with |- cmd _ _ _ _ ?l _ => l end in
+      apply atleastonce_localsmap
+        with (v0:=max_cycles)
+             (lt:=lt)
+             (invariant:=
+                fun i tr' m' l' =>
+                  exists (s' : state) is_valid,
+                    (* s' is the state for the new trace *)
+                    execution (p:=state_machine_parameters) tr' s'
+                    (* as long as the loop continues, we keep setting is_valid to
+                       0, so locals are unchanged until the loop breaks *)
+                    /\ l' = map.put l "is_valid" is_valid
+                    /\ (exists n',
+                          (* current state has the same control and expected
+                             output as the initial state, but a possibly different
+                             counter *)
+                          s' = BUSY (Build_busy_data ctrl out n')
+                          (* the counter matches the "measure" i *)
+                          /\ n' = i)
+                    (* memory is unaffected *)
+                    /\ (array scalar32 (word.of_Z 4) data_ptr data_arr ⋆ R)%sep m').
+      { apply lt_wf. }
+
+      { (* case in which the loop breaks immediately (cannot happen) *)
+        repeat straightline.
+        exfalso. (* proof by contradiction *)
+
+        repeat lazymatch goal with
+               | v := word.of_Z 0 |- _ => subst v
+                    | br := if word.eqb _ (word.of_Z 0) then _ else _ |- _ => subst br
+               end.
+        rewrite @word.unsigned_eqb in * by typeclasses eauto.
+        autorewrite with push_unsigned in *.
+        destruct_one_match_hyp_of_type bool; congruence. }
+
+      { (* proof that invariant holds at loop start *)
+        do 2 eexists; ssplit;
+        lazymatch goal with
+        | |- execution _ _ => eassumption
+        | |- (?x <= ?x)%nat => reflexivity
+        | |- ?x = ?x => reflexivity
+        | |- sep _ _ _ => eassumption
+        | |- _ = map.put _ _ _ => symmetry; solve [apply map.put_put_same]
+        | |- output_matches_state _ _ =>
+          cbv [output_matches_state] in *;
+          destruct_one_match; solve [eauto]
+        | _ => idtac
+        end; [ ].
+        eauto. }
+
+      { (* invariant holds through loop (or postcondition holds, if loop breaks) *)
+        intros; logical_simplify; subst.
+        repeat straightline.
+
+        (* Call aes_data_valid *)
+        straightline_call; eauto; [ ].
+
+        (* simplify guarantees *)
+        logical_simplify; subst.
+        cbn [read_step reg_category] in *.
+        destruct_one_match_hyp.
+
+        { (* case in which the status is now DONE; break *)
+          repeat straightline.
+          { (* continuation case -- contradiction *)
+            exfalso.
+            cbv [status_matches_state] in *.
+            repeat invert_bool.
+            simplify_implicits.
+            lazymatch goal with
+            | br := if word.eqb _ (word.of_Z 0) then _ else _,
+                    H : word.unsigned br <> 0 |- _ =>
+                    subst br; apply H
+            end.
+            push_unsigned.
+            destruct_one_match; subst; try reflexivity; [ ].
+            (* TODO: add to invert_bool *)
+            lazymatch goal with
+            | H:true = negb _ |- _ => symmetry in H; apply Bool.negb_true_iff in H
+            end.
+            congruence. }
+          { (* break case *)
+
+            (* Call aes_data_get *)
+            straightline_call; eauto; try reflexivity; [ ].
+
+            (* simplify guarantees *)
+            logical_simplify; subst.
+
+            (* postcondition *)
+            repeat straightline.
+            ssplit; eauto. } }
+
+        { (* case in which the state is still BUSY *)
+          intros; logical_simplify.
+          destruct_one_match_hyp; [ contradiction | subst ].
+          repeat straightline.
+
+          { (* continuation case *)
+            cbv [Markers.split].
+            match goal with |- exists v, _ /\ (v < S ?n)%nat => exists n end.
+            split; [ | lia ].
+
+            (* invariant still holds *)
+            do 2 eexists; ssplit;
+              lazymatch goal with
+              | |- execution _ _ => eassumption
+              | |- sep _ _ _ => eassumption
+              | |- @eq map.rep ?l1 ?l2 =>
+                subst1_map l1;
+                  lazymatch goal with
+                  | |- @eq map.rep ?l1 ?l2 =>
+                    subst1_map l1
+                  end;
+                  apply map.put_put_same
+              | _ => eauto
+              end. }
+          { (* break case -- contradiction *)
+            exfalso.
+            cbv [status_matches_state] in *.
+            repeat invert_bool; try congruence; [ ].
+            simplify_implicits.
+            lazymatch goal with
+            | H : word.eqb _ _ = negb (is_flag_set ?x ?flag),
+                  H' : is_flag_set ?x ?flag = _ |- _ =>
+              rewrite H' in H; cbn [negb] in H
+            end.
+            lazymatch goal with
+            | br := if word.eqb ?x (word.of_Z 0) then _ else _,
+                    Heq : word.eqb ?x (word.of_Z 0) = _,
+                          Hz : word.unsigned br = 0 |- _ =>
+                    subst br; rewrite Heq in Hz;
+                      autorewrite with push_unsigned in Hz
+            end.
+            discriminate. } } } }
+
+    { (* case in which the initial state is DONE *)
+
+      (* use output_matches_state precondition *)
+      lazymatch goal with
+      | H : ?data = done_data_from_output (done_ctrl ?data) out |- _ =>
+        cbv [done_data_from_output] in H; destruct data;
+        cbn [AesSemantics.done_ctrl
+               AesSemantics.done_data_out0
+               AesSemantics.done_data_out1
+               AesSemantics.done_data_out2
+               AesSemantics.done_data_out3] in *;
+        inversion H; clear H; subst
+      end.
+
+      (* while loop will run exactly once *)
+      eapply unroll_while with (iterations:=1%nat). cbn [repeat_logic_step].
+      repeat straightline.
+
+      (* prove that we do enter the while loop *)
+      ssplit;
+        [ subst_lets; rewrite word.eqb_eq by reflexivity;
+          push_unsigned; congruence | ].
+
       repeat straightline.
 
       (* Call aes_data_valid *)
@@ -1738,201 +1768,35 @@ Section Proofs.
 
       (* simplify guarantees *)
       logical_simplify; subst.
+      cbn [read_step reg_category] in *.
+      cbv [status_matches_state] in *.
+      logical_simplify; subst.
+      repeat invert_bool; try congruence; [ ].
+      simplify_implicits.
       lazymatch goal with
-      | H : execution (_ :: _) _ |- _ =>
-        pose proof H;
-        apply invert1_execution in H; logical_simplify
+      | H : word.eqb _ _ = negb (is_flag_set ?x ?flag),
+            H' : is_flag_set ?x ?flag = _ |- _ =>
+        rewrite H' in H; cbn [negb] in H;
+          apply word.eqb_false in H
       end.
-      invert_step; subst.
-      cbn [parameters.reg_addr parameters.write_step parameters.read_step
-                               state_machine_parameters] in *.
-      infer; subst.
-      (* assert that the register address we just read is STATUS *)
-      lazymatch goal with
-      | H : reg_addr ?r = AES_STATUS |- _ =>
-        apply (reg_addr_unique r STATUS) in H; subst
-      end.
-      invert_read_step; infer; subst; try discriminate;
-        (* get rid of cases that are not BUSY or DONE *)
-        try lazymatch goal with
-            | H : output_matches_state _ _ |- _ =>
-              cbv [output_matches_state] in H; contradiction H
-            end;
-        (* three cases left : BUSY -> DONE, BUSY -> BUSY, DONE -> DONE *)
-        [ | | ].
 
-      { (* case in which the state was BUSY, but is now DONE *)
-        repeat straightline.
-        { (* continuation case -- contradiction *)
-          exfalso.
-          cbv [status_matches_state] in *.
-          repeat invert_bool.
-          simplify_implicits.
-          lazymatch goal with
-          | br := if word.eqb _ (word.of_Z 0) then _ else _,
-                  H : word.unsigned br <> 0 |- _ =>
-                  subst br; apply H
-          end.
-          push_unsigned.
-          destruct_one_match; subst; try reflexivity; [ ].
-          (* TODO: add to invert_bool *)
-          lazymatch goal with
-          | H:true = negb _ |- _ => symmetry in H; apply Bool.negb_true_iff in H
-          end.
-          congruence. }
-        { (* break case *)
+      repeat straightline.
 
-          (* Call aes_data_get *)
-          straightline_call; eauto using nregs_populated_set_out_regs; [ ].
-          repeat straightline.
-          logical_simplify; subst.
-          lazymatch goal with
-          | H : execution (_ :: _) _ |- _ =>
-            apply invert1_execution in H; logical_simplify
-          end.
-          infer; subst.
-          (* assert that the register address we just read is STATUS *)
-          lazymatch goal with
-          | H : parameters.reg_addr ?r = AES_STATUS |- _ =>
-            replace AES_STATUS with (reg_addr STATUS) in H
-              by (cbn [reg_addr]; subst_lets; ring);
-              apply reg_addr_unique in H; try subst r
-          end.
-          cbn [parameters.reg_addr parameters.write_step parameters.read_step
-                                   state_machine_parameters] in *.
-          invert_read_step; subst; try discriminate; [ ].
-          infer.
+      (* prove the loop breaks *)
+      ssplit;
+        [ subst_lets; simplify_implicits;
+          destruct_one_match; push_unsigned; congruence | ].
 
-          (* postcondition *)
-          lazymatch goal with
-          | H : output_matches_state ?out _ |- context [?out] =>
-            cbv [output_matches_state] in H; subst
-          end.
-          cbv [reg_lookup set_out_regs] in *.
-          repeat lazymatch goal with
-                 | H : map.get (map.put _ ?k _) ?k = _ |- _ => rewrite map.get_put_same in H
-                 | H : map.get (map.put _ _ _) _ = _ |- _ =>
-                   rewrite map.get_put_diff in H by (apply reg_addr_neq; congruence)
-                 | H : context [map.remove (map.put _ ?k _) ?k] |- _ =>
-                   rewrite map_remove_put_same in H
-                 | H : context [map.remove (map.put _ _ _) _] |- _ =>
-                   rewrite map_remove_put_diff in H by (apply reg_addr_neq; congruence)
-                 | H : Some _ = Some _ |- _ => inversion H; clear H; subst
-                 end.
-          cbn [get_register_state].
-          ssplit; eauto. } }
+      repeat straightline.
 
-      { (* case in which the state was BUSY and is still BUSY *)
-        repeat straightline.
-        { (* continuation case *)
-          cbn [max_iterations]. cbv [Markers.split].
-          match goal with |- exists v, _ /\ (v < S ?n)%nat => exists n end.
-          split; [ | lia ].
+      (* Call aes_data_get *)
+      straightline_call; eauto; try reflexivity; [ ].
 
-          (* invariant still holds *)
-          do 2 eexists; ssplit;
-            lazymatch goal with
-            | |- execution _ _ => eassumption
-            | |- max_iterations _ = _ => reflexivity
-            | |- sep _ _ _ => eassumption
-            | |- @eq map.rep ?l1 ?l2 =>
-              subst1_map l1;
-                lazymatch goal with
-                | |- @eq map.rep ?l1 ?l2 =>
-                  subst1_map l1
-                end;
-                apply map.put_put_same
-            | |- exists n, ?f ?x = ?f n => exists x; reflexivity
-            | |- output_matches_state _ _ =>
-              cbv [output_matches_state] in *; solve [eauto]
-            | _ => idtac
-            end. }
-        { (* break case -- contradiction *)
-          exfalso.
-          cbv [status_matches_state] in *.
-          repeat invert_bool; try congruence; [ ].
-          lazymatch goal with
-          | H : word.eqb _ _ = negb (is_flag_set ?x ?flag),
-                H' : is_flag_set ?x ?flag = _ |- _ =>
-            rewrite H' in H; cbn [negb] in H
-          end.
-          simplify_implicits.
-          lazymatch goal with
-          | br := if word.eqb ?x (word.of_Z 0) then _ else _,
-                  Heq : word.eqb ?x (word.of_Z 0) = _,
-                  Hz : word.unsigned br = 0 |- _ =>
-                  subst br; rewrite Heq in Hz;
-                    autorewrite with push_unsigned in Hz
-          end.
-          discriminate. } }
+      (* simplify guarantees *)
+      logical_simplify; subst.
 
-      { (* case in which the state was DONE to begin with *)
-        repeat straightline.
-        { (* continuation case -- contradiction *)
-          exfalso.
-          cbv [status_matches_state] in *.
-          repeat invert_bool.
-          simplify_implicits.
-          lazymatch goal with
-          | br := if word.eqb _ (word.of_Z 0) then _ else _,
-                  H : word.unsigned br <> 0 |- _ =>
-                  subst br; apply H
-          end.
-          push_unsigned.
-          destruct_one_match; subst; try reflexivity; [ ].
-          (* TODO: add to invert_bool *)
-          lazymatch goal with
-          | H:true = negb _ |- _ => symmetry in H; apply Bool.negb_true_iff in H
-          end.
-          congruence. }
-        { (* break case *)
-
-          (* Call aes_data_get *)
-          straightline_call; eauto;
-          lazymatch goal with
-          | |- nregs_populated ?rs DataOutReg = _ =>
-            erewrite <-(output_matches_state_set_out_regs rs) by eassumption;
-            solve [eapply nregs_populated_set_out_regs]
-          | _ => idtac
-          end; [ ].
-          repeat straightline.
-          logical_simplify; subst.
-          lazymatch goal with
-          | H : execution (_ :: _) _ |- _ =>
-            apply invert1_execution in H; logical_simplify
-          end.
-          infer; subst.
-          (* assert that the register address we just read is STATUS *)
-          lazymatch goal with
-          | H : parameters.reg_addr ?r = AES_STATUS |- _ =>
-            replace AES_STATUS with (reg_addr STATUS) in H
-              by (cbn [reg_addr]; subst_lets; ring);
-              apply reg_addr_unique in H; try subst r
-          end.
-          cbn [parameters.reg_addr parameters.write_step parameters.read_step
-                                   state_machine_parameters] in *.
-          invert_read_step; subst; try discriminate; [ ].
-          infer.
-
-          (* postcondition *)
-          lazymatch goal with
-          | H : output_matches_state ?out _ |- context [?out] =>
-            cbv [output_matches_state] in H; subst
-          end.
-          cbv [reg_lookup set_out_regs] in *. logical_simplify.
-          repeat lazymatch goal with
-                 | H : map.get (map.put _ ?k _) ?k = _ |- _ => rewrite map.get_put_same in H
-                 | H : map.get (map.put _ _ _) _ = _ |- _ =>
-                   rewrite map.get_put_diff in H by (apply reg_addr_neq; congruence)
-                 | H : context [map.remove (map.put _ ?k _) ?k] |- _ =>
-                   rewrite map_remove_put_same in H
-                 | H : context [map.remove (map.put _ _ _) _] |- _ =>
-                   rewrite map_remove_put_diff in H by (apply reg_addr_neq; congruence)
-                 | H1 : map.get ?m ?k = Some _, H2 : map.get ?m ?k = Some _ |- _ =>
-                   rewrite H1 in H2
-                 | H : Some _ = Some _ |- _ => inversion H; clear H; subst
-                 end.
-          cbn [get_register_state].
-          ssplit; eauto. } } }
+      (* postcondition *)
+      repeat straightline.
+      ssplit; eauto. }
   Qed.
 End Proofs.
